updating

current/ThreeSatReduction.v
@@ -10,24 +10,26 @@ Export ListNotations.
 Require Export Arith.
 Require Export Arith.EqNat.  
 Require Export hetList. 
+Require Export Coq.Program.Equality. 
 
 Definition bvar := nat. (*boolean variables*)
 Definition vvar := nat. (*vertex variables*)
 Definition colors := nat. (*colors for graph vertices*) 
 Definition edge : Type := prod vvar vvar. (*graph edges*)
-
+ 
 (*boolean formula (n is the number of variables*)
-Inductive bformula : Type :=
-|pos :  bvar -> bformula 
-|neg : bvar -> bformula
-|conjForm : bformula -> bformula -> bformula
-|disjForm : bformula -> bformula -> bformula. 
+Inductive atom : Type := pos : bvar -> atom | neg : bvar -> atom. 
+
+Definition bformula := list (atom * atom * atom). 
+
+Inductive atomWF (n:nat) : atom -> Prop :=
+|posWF : forall x, x < n -> atomWF n (pos x)
+|negWF : forall x, x < n -> atomWF n (neg x). 
 
 Inductive bformulaWF (n:nat) : bformula -> Prop :=
-|posWF : forall x, x < n -> bformulaWF n (pos x)
-|negWF : forall x, x < n -> bformulaWF n (neg x)
-|conjWF : forall F1 F2, bformulaWF n F1 -> bformulaWF n F2 -> 
-                   bformulaWF n (conjForm F1 F2).
+|consWF : forall a1 a2 a3 tl, atomWF n a1 -> atomWF n a2 -> atomWF n a3 -> 
+                         bformulaWF n tl -> bformulaWF n ((a1,a2,a3)::tl)
+|nilWF : bformulaWF n nil. 
 
 (*graph*)
 Inductive graph : Type :=
@@ -41,12 +43,15 @@ Inductive graphWF (n:nat) : graph -> Prop :=
 |unionWF : forall G1 G2, graphWF n G1 -> graphWF n G2 -> graphWF n (gunion G1 G2). 
 
 (*Specificaion of SAT' satisfiability*)
+
+Inductive atomSAT : list (bvar * bool) -> atom -> Prop :=
+|satp : forall eta u, In (u, true) eta -> atomSAT eta (pos u)
+|satn : forall eta u, In (u, false) eta -> atomSAT eta (neg u). 
+
 Inductive SAT' : list (bvar * bool) -> bformula -> Prop :=
-|satp : forall eta u, In (u, true) eta -> SAT' eta (pos u)
-|satn : forall eta u, In (u, false) eta -> SAT' eta (neg u)
-|satConj : forall eta F1 F2, SAT' eta F1 -> SAT' eta F2 -> SAT' eta (conjForm F1 F2)
-|satDisj1 : forall eta F1 F2, SAT' eta F1 -> SAT' eta (disjForm F1 F2)
-|satDij2 : forall eta F1 F2, SAT' eta F2 -> SAT' eta (disjForm F1 F2).
+|satCons : forall a1 a2 a3 tl eta, atomSAT eta a1 -> atomSAT eta a2 -> atomSAT eta a3 ->
+                            SAT' eta tl -> SAT' eta ((a1,a2,a3)::tl)
+|satNil : forall eta, SAT' eta nil. 
 
 Fixpoint setVars n eta F :=
   match n with
@@ -87,91 +92,80 @@ an edge from that x to to the vertex variable provided (X)*)
 Inductive connectX : list (bvar * vvar * vvar * vvar) -> list bvar ->
                            vvar -> graph -> Prop :=
 |connectXNil : forall Gamma X, connectX Gamma nil X emptyGraph
-|connectX_vtx : forall Gamma Delta u v v' x' X G, 
-                  In (u, v, v', x') Gamma -> connectX Gamma Delta X G -> 
-                  connectX Gamma (u::Delta) X (newEdge X x' G). 
+|connectX_vtx : forall Gamma Delta u X G, 
+                  In (u, 3*u, 3*u+1, 3*u+2) Gamma -> connectX Gamma Delta X G -> 
+                  connectX Gamma (u::Delta) X (newEdge X (3*u+2) G). 
 
 (*Same as above for makes edges to v and v' rather than x*)
 Inductive connectV : list (bvar * vvar * vvar * vvar) -> list bvar ->
                       vvar -> graph -> Prop :=
 |connectV_nil : forall Gamma X, connectV Gamma nil X emptyGraph
-|connectV_vtx : forall Gamma Delta u v v' x' X G, 
-                  In (u, v, v', x') Gamma -> connectV Gamma Delta X G ->
-                  connectV Gamma (u::Delta) X (newEdge X v (newEdge X v' G)). 
+|connectV_vtx : forall Gamma Delta u X G, 
+                  In (u, 3*u, 3*u+1, 3*u+2) Gamma -> connectV Gamma Delta X G ->
+                  connectV Gamma (u::Delta) X (newEdge X (3*u) (newEdge X (3*u+1) G)). 
 
 Inductive vars_to_clique : list (bvar * vvar * vvar * vvar) -> list bvar ->
                            graph -> Prop :=
 |vars2cliqueNil : forall Gamma, vars_to_clique Gamma nil emptyGraph
-|vars2cliqueVTX : forall Gamma Delta u v v' x G1 G2 G3 G4, 
-         In (u,v,v',x) Gamma -> vars_to_clique Gamma Delta G1 ->
-         connectX Gamma Delta v G2 -> connectX Gamma Delta v' G3 ->
-         connectV Gamma Delta x G4 ->
+|vars2cliqueVTX : forall Gamma Delta u G1 G2 G3 G4, 
+         In (u,3*u,3*u+1,3*u+2) Gamma -> vars_to_clique Gamma Delta G1 ->
+         connectX Gamma Delta (3*u) G2 -> connectX Gamma Delta (3*u+1) G3 ->
+         connectV Gamma Delta (3*u+2) G4 ->
          vars_to_clique Gamma (u::Delta) (gunion G1 (gunion G2 (gunion G3 G4))). 
 
 Inductive clique : list (bvar * vvar * vvar * vvar) -> list bvar ->
                    graph -> Prop :=
 |clique_empty : forall Gamma, clique Gamma nil emptyGraph
-|clique_vtx : forall Gamma u v v' x Delta G1 G2, 
-                In (u,v,v',x) Gamma -> clique Gamma Delta G1 -> connectX Gamma Delta x G2 ->
+|clique_vtx : forall Gamma u Delta G1 G2, 
+                In (u,3*u,3*u+1,3*u+2) Gamma -> clique Gamma Delta G1 -> connectX Gamma Delta (3*u+2) G2 ->
                 clique Gamma (u::Delta) (gunion G1 G2). 
 
 (*convert base (Gamma; Delta |- C Downarrow G*)
 Inductive convert_base : list (bvar * vvar * vvar * vvar) -> list bvar ->
                          colors -> graph -> Prop :=
 |conv'''_base : forall Gamma C, convert_base Gamma nil C emptyGraph
-|conv'''_cont : forall Gamma Delta u v v' x C G,
-                  In (u,v,v',x) Gamma -> convert_base Gamma Delta C G ->
-                  convert_base Gamma (u::Delta) C (newEdge C v (newEdge C v' G)). 
+|conv'''_cont : forall Gamma Delta u C G,
+                  In (u,3*u,3*u+1,3*u+2) Gamma -> convert_base Gamma Delta C G ->
+                  convert_base Gamma (u::Delta) C (newEdge C (3*u) (newEdge C (3*u+1) G)). 
 
 (*mkEdge c u v v' e (determines if the edge from c goes to v or v')*)
-Inductive mkEdge : vvar -> bformula -> vvar -> vvar -> edge -> Prop :=
+Inductive mkEdge : vvar -> atom -> vvar -> vvar -> edge -> Prop :=
 |mkPos : forall c u v v', mkEdge c (pos u) v v' (c, v)
 |mkNeg : forall c u v v', mkEdge c (neg u) v v' (c, v'). 
 
 Inductive convFormula (c:vvar) : list (bvar * vvar * vvar * vvar) -> list bvar ->
-                        bformula -> graph -> Prop := 
-|conv'' : forall Gamma Delta u1 u2 u3 v1 v2 v3 v1' v2' v3' x1 x2 x3 G e1 e2 e3 p1 p2 p3, 
-            In (u1,v1,v1',x1) Gamma -> In (u2,v2,v2',x2) Gamma -> In (u3,v3,v3',x3) Gamma ->
-            convert_base Gamma Delta c G -> mkEdge c p1 v1 v1' e1 -> mkEdge c p2 v2 v2' e2 ->
-            mkEdge c p3 v3 v3' e3 -> 
-            convFormula c Gamma (u1::u2::u3::Delta) (disjForm p1 (disjForm p2 p3))
+                        (atom * atom * atom) -> graph -> Prop := 
+|conv'' : forall Gamma Delta u1 u2 u3 G e1 e2 e3 p1 p2 p3, 
+            In (u1,3*u1,3*u1+1,3*u1+2) Gamma -> In (u2,3*u2,3*u2+1,3*u2+2) Gamma -> In (u3,3*u3,3*u3+1,3*u3+2) Gamma ->
+            convert_base Gamma Delta c G -> mkEdge c p1 (3*u1) (3*u1+1) e1 -> mkEdge c p2 (3*u2) (3*u2+1) e2 ->
+            mkEdge c p3 (3*u3) (3*u3+1) e3 -> 
+            convFormula c Gamma (u1::u2::u3::Delta) (p1, p2, p3)
                         (newE [e1;e2;e3] G)
 . 
 
 (*Convert Stack of Continuations (Gamma; Delta |- K => G)*)
 Inductive convStack (i:vvar) : list (bvar * vvar * vvar * vvar) -> list bvar ->
-                      list bformula -> graph -> Prop :=
+                      bformula -> graph -> Prop :=
 |conv_base : forall Gamma Delta, convStack i Gamma Delta nil emptyGraph
 |conv_cons : forall Gamma Delta K F G1 G2, convStack (i+1) Gamma Delta K G1 -> convFormula i Gamma Delta F G2 ->
                               convStack i Gamma Delta (F::K) (gunion G1 G2)
 .
 
-(*Top Level Reduction (Gamma; Delta |- K o F => C C' G)*)
-Inductive reduce Gamma Delta : list bformula -> bformula -> nat -> nat -> graph -> Prop :=
-|convConj : forall K F F' C C' G, 
-              reduce Gamma Delta (F::K) F' C C' G ->
-              reduce Gamma Delta K (conjForm F F') C C' G
-|convV : forall K F1 F2 F3 G1 G2 G3 C,
-         convStack (length Gamma * 3) Gamma Delta ((disjForm F1 (disjForm F2 F3))::K) G1 ->
+(*Top Level Reduction (Gamma; Delta |- F => C C' G)*)
+Inductive reduce Gamma Delta : bformula -> nat -> graph -> Prop :=
+|convV : forall F G1 G2 G3 C,
+         convStack (length Gamma * 3) Gamma Delta F G1 ->
          clique Gamma Delta G2 -> vars_to_clique Gamma Delta G3 ->
-         reduce Gamma Delta K (disjForm F1 (disjForm F2 F3)) C C (gunion G1 (gunion G2 G3)).
+         reduce Gamma Delta F C (gunion G1 (gunion G2 G3)).
 
-Fixpoint buildCtxt n := 
-  match n with
-      |S n' => 
-       let (Gamma, Delta) := buildCtxt n'
-       in ((n', 3 * n', 3 * n' + 1, 3 * n' + 2)::Gamma, n'::Delta)
-      |0 => (nil, nil)
-  end.
+Inductive buildCtxt n : nat -> list (bvar*vvar*vvar*vvar) -> list bvar -> Prop :=
+|buildCons : forall Gamma Delta i, buildCtxt n (S i) Gamma Delta -> 
+                        buildCtxt n i ((i,3*i,3*i+1,3*i+2)::Gamma) (i::Delta)
+|buildNil : buildCtxt n n nil nil. 
 
-Definition Reduce F n : Prop := 
-  let (Gamma, Delta) := buildCtxt n
-  in reduce Gamma Delta nil F 0 (n+1) emptyGraph. 
-
-Theorem reductionInvariant : forall K F G C C' Delta Gamma, 
-                               reduce Gamma Delta K F C C' G -> C <= C'. 
+Theorem buildCtxtSanityChk : buildCtxt 3 0 [(0,0,1,2);(1,3,4,5);(2,6,7,8)] [0;1;2].
 Proof.
-  intros. induction H; omega. 
+  repeat constructor. 
 Qed. 
 
 Hint Constructors coloring. 
@@ -181,17 +175,6 @@ Proof.
   intros. induction H; eauto. econstructor; eauto; omega. 
 Qed. 
 
-Fixpoint stackSAT (eta:list (bvar * bool)) s :=
-  match s with
-      |b::bs => SAT' eta b /\ stackSAT eta bs 
-      |nil => True
-  end. 
-(*
-Let G be a graph; x1, x2, . . . , xn free vari- ables in G and u1,u2,...,un Boolean variables. Let ∆ = u1,u2,...,un and
-Γ = (u1, , ,x1),(u2, , ,x2),...,(un, , ,xn)3.
-If D :: Γ; ∆ ⊢ G CLIQUE and C ≥ c0 + n then there exists G :: η ⊢ G C COLORING where η = x1 → C1,x2 → C2,...,xn → Cn; Ci’s are distinct and Ci ≤ C.
-*)
-
 Ltac inv H := inversion H; subst; clear H.
 
 Ltac invertHyp :=
@@ -199,3 +182,286 @@ Ltac invertHyp :=
       |H:exists x, ?e |- _ => inv H; try invertHyp
       |H:?x /\ ?y |- _ => inv H; try invertHyp
   end.
+
+(*a generic specification of uniqueness (typically f is used to project
+**out of a tuple)*)
+Inductive genericUnique {A B :Type} (U:Ensemble B) (f:A -> B) : list A -> Prop :=
+|uniqueCons : forall hd tl, genericUnique (Add B U (f hd)) f tl ->
+                       ~ Ensembles.In _ U (f hd) -> genericUnique U f (hd::tl)
+|uniqueNil : genericUnique U f nil. 
+
+Inductive winner eta : atom -> bvar -> Prop :=
+|posWinner : forall x, In (x, true) eta -> winner eta (pos x) x
+|negWinner : forall x, In (x, false) eta -> winner eta (neg x) x. 
+
+Inductive setCs env : list (bvar*vvar*vvar*vvar) -> nat -> bformula -> 
+                        list (vvar * colors) -> list (bvar * bool) -> Prop := 
+|fstSAT : forall u eta eta' c i Gamma a1 a2 a3 F,
+            In (u, c) env -> winner eta a1 u -> setCs env Gamma (S i) F eta' eta ->
+            setCs env Gamma i ((a1, a2, a3)::F) ((i, c)::eta') eta
+|sndSAT : forall u eta eta' c i Gamma a1 a2 a3 F,
+            In (u, c) env -> winner eta a2 u -> setCs env Gamma (S i) F eta' eta ->
+            setCs env Gamma i ((a1, a2, a3)::F) ((i, c)::eta') eta
+|thirdSAT : forall u eta eta' c i Gamma a1 a2 a3 F,
+            In (u, c) env -> winner eta a3 u -> setCs env Gamma (S i) F eta' eta -> 
+            setCs env Gamma i ((a1, a2, a3)::F) ((i, c)::eta') eta
+|setCsDone : forall i Gamma eta eta', setCs env Gamma i nil eta'  eta. 
+
+
+(*N is the number of clauses in the boolean formula*)
+(*specifies how a graph environment is built out of a boolean formula
+**environment and reduction contexts*) 
+Inductive setVertices : list (bvar*vvar*vvar*vvar) -> nat -> nat ->
+                  list (vvar * colors) ->  list (bvar * bool) -> Prop :=
+|setVerticesT : forall u eta eta' C Gamma, 
+            setVertices Gamma C (S u) eta' eta -> u <= C -> 
+            setVertices ((u,3*u,3*u+1,3*u+2)::Gamma) C u 
+                  ((3*u,u)::(3*u+1,C)::(3*u+2,u)::eta') ((u,true)::eta)
+|setVerticesF : forall u eta eta' C Gamma, 
+            setVertices Gamma C (S u) eta' eta -> u <= C ->
+            setVertices ((u,3*u,3*u+1,3*u+2)::Gamma) C u
+                  ((3*u,C)::(3*u+1,u)::(3*u+2,u)::eta') ((u, false)::eta)
+|setVerticesNil : forall C u, setVertices nil C u nil nil.
+
+Theorem sanityCheck : setVertices [(0,0,1,2);(1,3,4,5);(2,6,7,8)]
+                            3 0  [(0,0);(1,3);(2,0);(3,3);(4,1);(5,1);(6,2);(7,3);(8,2)]
+                            [(0, true); (1, false); (2, true)].
+Proof.
+  repeat constructor.
+Qed. 
+
+Inductive valid : list (bvar*vvar*vvar*vvar) -> nat -> bformula -> 
+                  list (vvar * colors) -> list (bvar * bool) -> Prop :=
+|valid_ : forall Gamma C eta eta' eta'' F res, setVertices Gamma C 0 eta' eta -> 
+                          setCs eta' Gamma (3 * length Gamma) F eta'' eta ->
+                          res = eta' ++ eta'' -> 
+                          valid Gamma C F res eta. 
+
+Theorem sanityCheck' : 
+  valid [(0,0,1,2);(1,3,4,5);(2,6,7,8)]
+              3  [(neg 0, pos 1, pos 2)]
+              [(0,0);(1,3);(2,0);(3,3);(4,1);(5,1);(6,2);(7,3);(8,2);(9,0)]
+              [(0, true); (1, false); (2, true)].
+Proof.
+  econstructor. repeat econstructor. Focus 2. simpl. auto.
+  eapply thirdSAT. simpl. right. right. left. auto. constructor. simpl. 
+  auto. constructor. 
+Qed. 
+
+(*colors assigned to each of the xi's are unique*)
+Inductive uniqueGraphEnv S : list (vvar * colors) -> Prop :=
+|rConsUnique : forall (x:vvar) (y y' y'':colors) l, 
+                 uniqueGraphEnv (Add colors S y'') l ->
+                 uniqueGraphEnv S ((x,y)::(x+1,y')::(x+2,y'')::l)
+|rNilUnique : uniqueGraphEnv S nil. 
+
+(*Set addition commutes (probably defined elsewhere in the standard library)*)
+Theorem AddComm : forall (U:Type) S i i', Add U (Add U S i) i' = Add U (Add U S i') i. 
+Proof.
+  intros. apply Extensionality_Ensembles. unfold Same_set. unfold Included. 
+  split; intros. 
+  {inv H. inv H0. constructor. constructor. auto. inv H. unfold Add. 
+   apply Union_intror. constructor. inv H0. constructor. unfold Add. 
+   apply Union_intror. constructor. }
+  {inv H. inv H0. constructor. constructor. auto. inv H. unfold Add. 
+   apply Union_intror. constructor. inv H0. constructor. unfold Add. 
+   apply Union_intror. constructor. }
+Qed. 
+
+Theorem setVerticesUnique : forall Gamma eta eta' C S i, 
+                        setVertices Gamma C i eta' eta -> 
+                        (forall x, Ensembles.In _ S x -> x <= i) ->
+                        uniqueGraphEnv S eta'. 
+Proof.
+  intros. generalize dependent S. induction H; intros.  
+  {constructor. eapply IHsetVertices. intros. inv H2. apply H1 in H3. 
+   omega. inv H3. omega. }
+  {constructor. eapply IHsetVertices. intros. inv H2. apply H1 in H3. 
+   omega. inv H3. omega. }
+  {constructor. }
+Qed. 
+
+
+(*a valid graph environment assigns unique colors to each of the xs*)
+Theorem validUnique : forall Gamma eta eta' C S i F, 
+                        valid Gamma C F eta' eta -> 
+                        (forall x, Ensembles.In _ S x -> x >= i) ->
+                        uniqueGraphEnv S eta'. 
+Proof.
+  intros. inv H. apply setVerticesUnique with (S := Empty_set _) in H1. 
+  Focus 2. intros. inv H. 
+
+
+ generalize dependent S. induction H; intros.
+  {constructor. eapply IHvalid. intros. inv H3. apply H2 in H4. omega. inv H4. 
+   omega. }
+  {constructor. eapply IHvalid. intros. inv H3. apply H2 in H4. omega. inv H4. 
+   omega. }
+  {constructor. }
+Qed. 
+
+Ltac copy H := 
+  match type of H with
+      |?x => assert(x) by auto 
+  end. 
+
+Inductive uniqueLockstep {a b c d : Type} S1 S2 S3 S4 : list (a*b*c*d) -> Prop :=
+|uniqueLSCons : forall x1 x2 x3 x4 l, 
+                  uniqueLockstep (Add a S1 x1) (Add b S2 x2) (Add c S3 x3)
+                                 (Add d S4 x4) l -> ~ Ensembles.In _ S1 x1 ->
+                  ~ Ensembles.In _ S2 x2 -> ~ Ensembles.In _ S3 x3 ->
+                  ~ Ensembles.In _ S4 x4 ->
+                  uniqueLockstep S1 S2 S3 S4 ((x1,x2,x3,x4)::l)
+|uniqueLSNil : uniqueLockstep S1 S2 S3 S4 nil. 
+
+Theorem InLSUnique : forall (A B C D:Type) Gamma S1 S2 S3 S4 u v v' x u1 v1 v1' x1, 
+                       Ensembles.In A S1 u -> Ensembles.In B S2 v ->
+                       Ensembles.In C S3 v' -> Ensembles.In D S4 x ->
+                       In (u1,v1,v1',x1) Gamma -> uniqueLockstep S1 S2 S3 S4 Gamma -> 
+                       u <> u1 /\ v <> v1 /\ v' <> v1' /\ x <> x1. 
+Proof.
+  induction Gamma; intros. 
+  {inv H3. }
+  {copy H3. inv H3. 
+   {inv H5. inv H4. split. intros c; subst; contradiction. 
+    split. intros c; subst; contradiction. split; intros c; subst; contradiction. 
+    inv H4. eapply IHGamma. Focus 6. eauto. constructor. auto. 
+    constructor. auto. constructor. auto. constructor. auto. auto. }
+   {inv H5. inv H4. split. intros c. subst. contradiction. 
+    split. intros c; subst. contradiction. split; intros c; subst; contradiction. 
+    inv H4. eapply IHGamma. Focus 6. eauto. constructor. auto. constructor. auto. 
+    constructor. auto. constructor. auto. auto. }
+  }
+Qed. 
+
+Theorem uniqueLSNeq : forall Gamma (u u1:bvar) (v v' x v1 v1' x1:vvar) S1 S2 S3 S4, 
+                        In (u,v,v',x) Gamma -> In (u1,v1,v1',x1) Gamma ->
+                        uniqueLockstep S1 S2 S3 S4 Gamma -> u <> u1 ->
+                        v <> v1 /\ v' <> v1' /\ x <> x1. 
+Proof.
+  induction Gamma; intros. 
+  {inv H. }
+  {simpl in *. inv H. 
+   {inv H0. 
+    {inv H. exfalso. apply H2. auto. }
+    {inv H1. eapply InLSUnique in H7; eauto. Focus 2. unfold Add. apply Union_intror. 
+     constructor. Focus 2. apply Union_intror. constructor. Focus 2. 
+     apply Union_intror. constructor. Focus 2. apply Union_intror. constructor. 
+     invertHyp. eauto. }
+   }
+   {inv H0. 
+    {inv H1. eapply InLSUnique in H7; eauto. Focus 2. apply Union_intror.
+     constructor. Focus 2. apply Union_intror. constructor. Focus 2. 
+     apply Union_intror. constructor. Focus 2. apply Union_intror. constructor. 
+     invertHyp. auto. }
+    {inv H1. eapply IHGamma. Focus 3. eauto. eauto. eauto. auto. }
+   }
+  }
+Qed.
+ 
+Theorem InValid : forall u C Gamma i eta eta', 
+                    valid Gamma C i eta' eta -> In (u,3*u,3*u+1,3*u+2) Gamma -> 
+                    exists c, In (3*u+2,c) eta' /\ c <= C. 
+Proof.
+  intros. induction H. 
+  {inv H0. 
+   {inv H3. econstructor. simpl. auto. }
+   {eapply IHvalid in H3. invertHyp. exists x. split; simpl; auto. }
+  }
+  {inv H0. 
+   {inv H3. econstructor. simpl. auto. }
+   {eapply IHvalid in H3. invertHyp. exists x. split; simpl; auto. }
+  }
+  {inv H0. }
+Qed. 
+
+Theorem LSUniqueSubset : forall A B C D a b c d S1 S2 S3 S4 Gamma, 
+                           uniqueLockstep (Add A S1 a) (Add B S2 b) 
+                                          (Add C S3 c) (Add D S4 d) Gamma ->
+                           uniqueLockstep S1 S2 S3 S4 Gamma. 
+Proof.
+  intros. dependent induction H. 
+  {constructor. eapply IHuniqueLockstep; auto; try solve[rewrite AddComm; auto]. 
+   intros Contr. apply H0. constructor. auto. intros x. apply H1. constructor. auto. 
+   intros x. apply H2. constructor. auto. intros x. apply H3. constructor. auto. }
+  {constructor. }
+Qed. 
+ 
+Require Export Coq.Logic.Classical_Prop. 
+
+Theorem notDistr : forall A B, ~(A \/ B) <-> ~ A /\ ~ B. 
+Proof.
+  intros. split; intros. 
+  {unfold not in H. split. intros c. apply H. auto. intros c. apply H; auto. }
+  {unfold not in H. invertHyp. intros c. inv c. auto. auto. }
+Qed. 
+
+Theorem genericUniqueNotIn : forall A B S (f:A -> B) (u:A) Delta,
+                               Ensembles.In _ S (f u) -> 
+                               genericUnique S f Delta ->  ~ In u Delta. 
+Proof.
+  intros. induction H0. 
+  {assert(u=hd \/ u <> hd). apply classic. inv H2. 
+   {contradiction. }
+   {simpl. rewrite notDistr. split. auto. apply IHgenericUnique. constructor. auto. }
+  }
+  {intros c. auto. }
+Qed. 
+
+Theorem genericUniqueSubset : forall A B (f:A -> B) U u Delta, 
+                                genericUnique (Add B U u) f Delta ->
+                                genericUnique U f Delta. 
+Proof.
+  intros. dependent induction H. 
+  {subst. constructor. eapply IHgenericUnique. rewrite AddComm. auto. 
+   intros c. apply H0. constructor. auto. }
+  {constructor. }
+Qed. 
+
+Ltac invertTupEq := 
+  match goal with
+      |H:(?x1,?x2) = (?y1,?y2) |- _ => inv H; try invertTupEq
+      |H:(?x1,?x2,?x3) = (?y1,?y2,?y3) |- _ => inv H; try invertTupEq
+      |H:(?x1,?x2,?x3,?x4) = (?y1,?y2,?y3,?y4) |- _ => inv H; try invertTupEq
+  end. 
+
+Ltac invUnique :=
+  match goal with
+      |H:uniqueLockstep ?S1 ?s2 ?s3 ?s4 (?x::?y) |- _ => inv H; try invUnique
+      |H:genericUnique ?U ?f (?x::?y) |- _ => inv H; try invUnique
+  end. 
+
+Theorem ltValid : forall Gamma eta' eta c u C j U S1 S2 S3 S4, 
+              valid Gamma C j eta' eta -> uniqueLockstep S1 S2 S3 S4 Gamma ->
+              genericUnique U (fun a=>match a with (x,y) => x end) eta' ->
+              In (u,3*u,3*u+1,3*u+2) Gamma -> In (3*u+2,c) eta' -> c <= j. 
+Proof.
+  intros. genDeps {{ c; u; U; S1; S2; S3; S4 }}. induction H; intros. 
+  {destruct (eq_nat_dec u u0). 
+   {subst. inv H4. 
+    {inv H5. invertTupEq. omega. inv H4. invertTupEq. omega. inv H5. invertTupEq. omega. 
+     assert(~ In (3 * S i + 2, c) eta'). invUnique. 
+     eapply genericUniqueNotIn. Focus 2. eauto. apply Union_intror.
+     constructor. contradiction. }
+    {invUnique. eapply InLSUnique in H10; try solve[apply Union_intror; constructor]. 
+     Focus 2. eauto. invertHyp. exfalso. apply H2. auto. }
+   }
+   {inv H4. invertTupEq. omega. inv H5. invertTupEq. omega. inv H1. invertTupEq. omega. 
+    inv H4. invertTupEq. omega. invUnique. eapply IHvalid in H10; eauto. }
+  }
+  { destruct (eq_nat_dec u u0). 
+   {subst. inv H4. 
+    {inv H5. invertTupEq. omega. inv H4. invertTupEq. omega. inv H5. invertTupEq. omega. 
+     assert(~ In (3 * S i + 2, c) eta'). invUnique. 
+     eapply genericUniqueNotIn. Focus 2. eauto. apply Union_intror.
+     constructor. contradiction. }
+    {invUnique. eapply InLSUnique in H10; try solve[apply Union_intror; constructor]. 
+     Focus 2. eauto. invertHyp. exfalso. apply H2. auto. }
+   }
+   {inv H4. invertTupEq. omega. inv H5. invertTupEq. omega. inv H1. invertTupEq. omega. 
+    inv H4. invertTupEq. omega. invUnique. eapply IHvalid in H10; eauto. }
+  }
+  {inv H3. }
+Qed. 
+
+
