current/cliqueColorable.v
@@ -1,274 +1,70 @@
-Require Import ThreeSatReduction. 
+Require Export ThreeSatReduction.  
 
-(*a generic specification of uniqueness (typically f is used to project
-**out of a tuple)*)
-Inductive genericUnique {A B :Type} (U:Ensemble B) (f:A -> B) : list A -> Prop :=
-|uniqueCons : forall hd tl, genericUnique (Add B U (f hd)) f tl ->
-                       ~ Ensembles.In _ U (f hd) -> genericUnique U f (hd::tl)
-|uniqueNil : genericUnique U f nil. 
-
-(*specifies how a graph environment is built out of a boolean formula
-**environment and reduction contexts*)
-Inductive valid : list (bvar*vvar*vvar*vvar) -> nat -> nat ->
-                        list (vvar * colors) -> list (bvar * bool) -> Prop :=
-|validF : forall u (v v' : vvar) x eta eta' C i Gamma, 
-            valid Gamma C (S i) eta' eta -> i <= C -> 
-            valid ((u,v,v',x)::Gamma) C i ((v,i)::(v',0)::(x,i)::eta')((u,true)::eta)
-|validT : forall u (v v' : vvar) x eta eta' i C Gamma, 
-            valid Gamma C (S i) eta' eta -> i <= C -> 
-            valid ((u,v,v',x)::Gamma) C i ((v,0)::(v',i)::(x,i)::eta') ((u, false)::eta)
-|validNil : forall C i, valid nil C i nil nil.
-
-(*colors assigned to each of the xi's are unique*)
-Inductive uniqueGraphEnv S : list (vvar * colors) -> Prop :=
-|rConsUnique : forall (x x' x'':vvar) (y y' y'':colors) l, 
-                 uniqueGraphEnv (Add colors S y'') l ->
-                 uniqueGraphEnv S ((x,y)::(x',y')::(x'',y'')::l)
-|rNilUnique : uniqueGraphEnv S nil. 
-
-(*Set addition commutes (probably defined elsewhere in the standard library)*)
-Theorem AddComm : forall (U:Type) S i i', Add U (Add U S i) i' = Add U (Add U S i') i. 
-Proof.
-  intros. apply Extensionality_Ensembles. unfold Same_set. unfold Included. 
-  split; intros. 
-  {inv H. inv H0. constructor. constructor. auto. inv H. unfold Add. 
-   apply Union_intror. constructor. inv H0. constructor. unfold Add. 
-   apply Union_intror. constructor. }
-  {inv H. inv H0. constructor. constructor. auto. inv H. unfold Add. 
-   apply Union_intror. constructor. inv H0. constructor. unfold Add. 
-   apply Union_intror. constructor. }
-Qed. 
-
-(*a valid graph environment assigns unique colors to each of the xs*)
-Theorem validUnique' : forall Gamma eta eta' C i U, 
-                        valid Gamma C (S i) eta' eta -> uniqueGraphEnv U eta' -> 
-                        uniqueGraphEnv (Add colors U i) eta'.
-Proof.
-  intros. generalize dependent U. induction H; intros. 
-  {constructor. rewrite AddComm. apply IHvalid. inv H1. auto. }
-  {inv H1. constructor. rewrite AddComm. eauto. }
-  {constructor. }
-Qed. 
-
-Theorem validUnique : forall Gamma eta eta' C S i, 
-                        valid Gamma C i eta' eta -> 
-                        uniqueGraphEnv S eta'. 
-Proof.
-  intros. induction H. 
-  {constructor. eapply validUnique'; eauto. }
-  {constructor. eapply validUnique'; eauto. }
-  {constructor. }
-Qed. 
-
-Ltac copy H := 
-  match type of H with
-      |?x => assert(x) by auto 
-  end. 
-
-Inductive uniqueLockstep {a b c d : Type} S1 S2 S3 S4 : list (a*b*c*d) -> Prop :=
-|uniqueLSCons : forall x1 x2 x3 x4 l, 
-                  uniqueLockstep (Add a S1 x1) (Add b S2 x2) (Add c S3 x3)
-                                 (Add d S4 x4) l -> ~ Ensembles.In _ S1 x1 ->
-                  ~ Ensembles.In _ S2 x2 -> ~ Ensembles.In _ S3 x3 ->
-                  ~ Ensembles.In _ S4 x4 ->
-                  uniqueLockstep S1 S2 S3 S4 ((x1,x2,x3,x4)::l)
-|uniqueLSNil : uniqueLockstep S1 S2 S3 S4 nil. 
-
-Theorem InLSUnique : forall (A B C D:Type) Gamma S1 S2 S3 S4 u v v' x u1 v1 v1' x1, 
-                       Ensembles.In A S1 u -> Ensembles.In B S2 v ->
-                       Ensembles.In C S3 v' -> Ensembles.In D S4 x ->
-                       In (u1,v1,v1',x1) Gamma -> uniqueLockstep S1 S2 S3 S4 Gamma -> 
-                       u <> u1 /\ v <> v1 /\ v' <> v1' /\ x <> x1. 
-Proof.
-  induction Gamma; intros. 
-  {inv H3. }
-  {copy H3. inv H3. 
-   {inv H5. inv H4. split. intros c; subst; contradiction. 
-    split. intros c; subst; contradiction. split; intros c; subst; contradiction. 
-    inv H4. eapply IHGamma. Focus 6. eauto. constructor. auto. 
-    constructor. auto. constructor. auto. constructor. auto. auto. }
-   {inv H5. inv H4. split. intros c. subst. contradiction. 
-    split. intros c; subst. contradiction. split; intros c; subst; contradiction. 
-    inv H4. eapply IHGamma. Focus 6. eauto. constructor. auto. constructor. auto. 
-    constructor. auto. constructor. auto. auto. }
-  }
-Qed. 
-
-Theorem uniqueLSNeq : forall Gamma (u u1:bvar) (v v' x v1 v1' x1:vvar) S1 S2 S3 S4, 
-                        In (u,v,v',x) Gamma -> In (u1,v1,v1',x1) Gamma ->
-                        uniqueLockstep S1 S2 S3 S4 Gamma -> u <> u1 ->
-                        v <> v1 /\ v' <> v1' /\ x <> x1. 
-Proof.
-  induction Gamma; intros. 
-  {inv H. }
-  {simpl in *. inv H. 
-   {inv H0. 
-    {inv H. exfalso. apply H2. auto. }
-    {inv H1. eapply InLSUnique in H7; eauto. Focus 2. unfold Add. apply Union_intror. 
-     constructor. Focus 2. apply Union_intror. constructor. Focus 2. 
-     apply Union_intror. constructor. Focus 2. apply Union_intror. constructor. 
-     invertHyp. eauto. }
-   }
-   {inv H0. 
-    {inv H1. eapply InLSUnique in H7; eauto. Focus 2. apply Union_intror.
-     constructor. Focus 2. apply Union_intror. constructor. Focus 2. 
-     apply Union_intror. constructor. Focus 2. apply Union_intror. constructor. 
-     invertHyp. auto. }
-    {inv H1. eapply IHGamma. Focus 3. eauto. eauto. eauto. auto. }
-   }
-  }
-Qed. 
-Theorem InValid : forall u v v' x C Gamma i eta eta', 
-                    valid Gamma C i eta' eta -> In (u,v,v',x) Gamma -> 
-                    exists c, In (x,c) eta' /\ c <= C. 
-Proof.
-  intros. induction H. 
-  {inv H0. 
-   {inv H2. simpl. exists i. split. auto. auto. }
-   {eapply IHvalid in H2. invertHyp. exists x1. split. simpl. 
-    right. eauto. auto. }
-  }
-  {inv H0. 
-   {inv H2. simpl. exists i. split. auto. auto. }
-   {eapply IHvalid in H2. invertHyp. exists x1. split. simpl. 
-    right. eauto. auto. }
-  }
-  {inv H0. }
-Qed. 
-
-Require Import Coq.Program.Equality. 
-
-Theorem LSUniqueSubset : forall A B C D a b c d S1 S2 S3 S4 Gamma, 
-                           uniqueLockstep (Add A S1 a) (Add B S2 b) 
-                                          (Add C S3 c) (Add D S4 d) Gamma ->
-                           uniqueLockstep S1 S2 S3 S4 Gamma. 
-Proof.
-  intros. dependent induction H. 
-  {constructor. eapply IHuniqueLockstep; auto; try solve[rewrite AddComm; auto]. 
-   intros Contr. apply H0. constructor. auto. intros x. apply H1. constructor. auto. 
-   intros x. apply H2. constructor. auto. intros x. apply H3. constructor. auto. }
-  {constructor. }
-Qed. 
- 
-Require Export Coq.Logic.Classical_Prop. 
-
-Theorem notDistr : forall A B, ~(A \/ B) <-> ~ A /\ ~ B. 
-Proof.
-  intros. split; intros. 
-  {unfold not in H. split. intros c. apply H. auto. intros c. apply H; auto. }
-  {unfold not in H. invertHyp. intros c. inv c. auto. auto. }
-Qed. 
-
-Theorem genericUniqueNotIn : forall A B S (f:A -> B) (u:A) Delta,
-                               Ensembles.In _ S (f u) -> 
-                               genericUnique S f Delta ->  ~ In u Delta. 
-Proof.
-  intros. induction H0. 
-  {assert(u=hd \/ u <> hd). apply classic. inv H2. 
-   {contradiction. }
-   {simpl. rewrite notDistr. split. auto. apply IHgenericUnique. constructor. auto. }
-  }
-  {intros c. auto. }
-Qed. 
-
-Theorem genericUniqueSubset : forall A B (f:A -> B) U u Delta, 
-                                genericUnique (Add B U u) f Delta ->
-                                genericUnique U f Delta. 
-Proof.
-  intros. dependent induction H. 
-  {subst. constructor. eapply IHgenericUnique. rewrite AddComm. auto. 
-   intros c. apply H0. constructor. auto. }
-  {constructor. }
-Qed. 
-
-Theorem ltValid : forall Gamma eta' eta c u v v' x C j, 
-              valid Gamma C j eta' eta -> 
-              In (u,v,v',x) Gamma -> In (x,c) eta' -> c >= j. 
-Proof.
-  intros. genDeps {{ c; x; u; v; v' }}. induction H; intros. 
-  {inv H2. 
-   {Admitted. 
-
-Theorem edgesNeq : forall eta' eta Gamma C i u v v' x u1 v1 v1' x1 S1 S2 S3 S4, 
-                     u <> u1 -> In (u,v,v',x) Gamma -> In (u1,v1,v1',x1) Gamma ->
+Theorem edgesNeq : forall eta' eta Gamma C i u U u1 S1 S2 S3 S4, 
+                     u <> u1 -> In (u,3*u,3*u+1,3*u+2) Gamma -> In (u1,3*u1,3*u1+1,3*u1+2) Gamma ->
                      valid Gamma C i eta' eta -> uniqueLockstep S1 S2 S3 S4 Gamma ->
-                     exists c1 c2, In (x,c1) eta' /\ In (x1, c2) eta' /\ c1 <> c2 /\
+                     genericUnique U (fun a=>match a with (x,y) => x end) eta' ->
+                     exists c1 c2, In (3*u+2,c1) eta' /\ In (3*u1+2, c2) eta' /\ c1 <> c2 /\
                               c1 <= C /\ c2 <= C. 
 Proof.
-  intros. genDeps {{ u;v;v';x;u1;v1;v1';x1 }}. induction H2; intros.
-  {inv H1. 
-   {inv H5. inv H4. 
-    {inv H1. exfalso. apply H0; auto. }
-    {inv H3. copy H1. eapply InValid in H1; eauto. invertHyp. 
-     exists x. exists i. split. simpl. auto. split. simpl. auto. split; auto. 
-     copy H2. eapply ltValid in H2; eauto.
-     eapply validUnique with (S:=Empty_set _)in H4. 
-     
- omega. }
+  intros. genDeps {{ u;u1;S1;S2;S3;S4;U }}. induction H2; intros.
+  {inv H1.  
+   {inv H6. 
+    {invertTupEq. omega. }
+    {invertTupEq. inv H3. copy H2. eapply InValid in H2; eauto. invertHyp. 
+     econstructor. econstructor. split. simpl. repeat right. eauto. split. 
+     simpl. auto. invUnique. eapply ltValid in H13; eauto.
+     split. omega. split; auto. }
    }
-   {inv H4.
-    {inv H1. inv H3. exists i. copy H5. eapply InValid in H5; eauto. invertHyp. 
-     exists x. split; simpl; auto. split. auto. split; auto. eapply ltValid in H2; eauto. 
-     omega. }
-    {inv H3. eapply IHvalid in H5; eauto. invertHyp. exists x3. exists x2. simpl. 
-     split; auto. eapply LSUniqueSubset; eauto. }
+   {inv H6. 
+    {invUnique. invertTupEq. exists (S i). copy H2. eapply InValid in H2; eauto. invertHyp. exists x. 
+     split; simpl; auto. split. auto. split; auto. eapply ltValid in H2; eauto. omega. }
+    {invUnique. eapply IHvalid in H7; eauto. invertHyp. exists x0. exists x. simpl. split; auto. }
    }
   }
-  {inv H1. 
-   {inv H5. inv H4. 
-    {inv H1. exfalso. apply H0; auto. }
-    {inv H3. copy H1. eapply InValid in H1; eauto. invertHyp. 
-     exists x. exists i. split. simpl. auto. split. simpl. auto. split; auto. admit. }
+  {inv H1.  
+   {inv H6. 
+    {invertTupEq. omega. }
+    {invertTupEq. inv H3. copy H2. eapply InValid in H2; eauto. invertHyp. 
+     econstructor. econstructor. split. simpl. repeat right. eauto. split. 
+     simpl. auto. invUnique. eapply ltValid in H13; eauto.
+     split. omega. split; auto. }
    }
-   {inv H4.
-    {inv H1. inv H3. eapply InValid in H5; eauto. invertHyp. exists i. exists x. 
-     split. simpl; auto. split. simpl; auto. split ;auto. 
-
- admit. }
-    {inv H3. eapply IHvalid in H5; eauto. invertHyp. exists x3. exists x2. simpl. 
-     split; auto. eapply LSUniqueSubset; eauto. }
+   {inv H6. 
+    {invUnique. invertTupEq. exists (S i). copy H2. eapply InValid in H2; eauto. invertHyp. exists x. 
+     split; simpl; auto. split. auto. split; auto. eapply ltValid in H2; eauto. omega. }
+    {invUnique. eapply IHvalid in H7; eauto. invertHyp. exists x0. exists x. simpl. split; auto. }
    }
   }
   {inv H0. }
 Qed. 
 
-Theorem connectXColorable : forall Gamma Delta G C eta eta' u v v' x S1 S2 S3 S4, 
+Theorem connectXColorable : forall Gamma Delta G C eta eta' U u S1 S2 S3 S4, 
                               uniqueLockstep S1 S2 S3 S4 Gamma -> 
-                              ~In u Delta -> valid Gamma C 1 eta' eta -> In (u,v,v',x) Gamma ->
-                              connectX Gamma Delta x G -> coloring eta' G C. 
+                              ~In u Delta -> valid Gamma C 1 eta' eta -> In (u,3*u,3*u+1,3*u+2) Gamma ->
+                              genericUnique U (fun a=>match a with (x,y) => x end) eta' ->
+                              connectX Gamma Delta (3*u+2) G -> coloring eta' G C. 
 Proof.
-  intros. genDeps {{ u; v; v'; eta; C; eta'}}. induction H3; intros. 
-  {constructor. }
-  {copy H1. eapply validUnique with (S := Empty_set _) in H5. 
+  intros. genDeps {{ eta; C; eta'}}. remember (3*u+2). induction H4; intros. 
+  {constructor. } 
+  {subst. copy H5. eapply validUnique with (S := Empty_set _) in H5. 
    destruct(eq_nat_dec u u0). 
-   {subst. simpl in H2. exfalso. apply H2. auto. }
-   {copy H1. eapply edgesNeq in H1; eauto. invertHyp. econstructor; eauto.
-    eapply IHconnectX; eauto. intros c. apply H2. simpl. right. auto. }
+   {subst. simpl in H2. exfalso. apply H0. simpl. auto. }
+   {copy H6. eapply edgesNeq in H6; eauto. invertHyp. econstructor; eauto.
+    eapply IHconnectX; eauto. intros c. apply H0. simpl. right. auto. }
+   intros. inv H7. 
   }
 Qed. 
 
-Theorem cliqueColorable : forall Gamma eta Delta C G eta' S1 S2 S3 S4 S5, 
+Theorem cliqueColorable : forall Gamma eta Delta C G eta' U S1 S2 S3 S4 S5, 
                             valid Gamma C 1 eta' eta -> 
                             uniqueLockstep S1 S2 S3 S4 Gamma ->
                             genericUnique S5 (fun x => x) Delta -> 
+                            genericUnique U (fun a=>match a with (x,y) => x end) eta' ->
                             clique Gamma Delta G -> coloring eta' G C. 
 Proof.
-  intros. genDeps {{ eta; C }}. induction H2; intros; auto. 
+  intros. genDeps {{ eta; C; U }}. induction H3; intros; auto. 
   {constructor. eapply IHclique; eauto. inv H1. eapply genericUniqueSubset; eauto. 
    eapply connectXColorable; eauto. inv H1. eapply genericUniqueNotIn. 
    Focus 2. eauto. simpl. apply Union_intror. constructor. }
 Qed. 
-
-Theorem KColorNPC : forall Gamma Delta K F C eta C' G eta',
-                      domainPostfix Delta Gamma -> reduce Gamma Delta K F C C' G -> 
-                      valid Gamma C' 1 eta' eta ->
-                      (stackSAT eta K /\ SAT' eta F <-> coloring eta' G C').
-Proof.
-  intros. split; intros. 
-  {generalize dependent eta'. induction H0; intros. 
-   {invertHyp. inv H4. apply IHreduce; auto. simpl. auto. }
-   {constructor. admit. constructor.
-    eapply cliqueColorable with (Gamma := Gamma)(S := Empty_set colors)(Delta := Delta); auto. 
-
-
-
