current/Main.v
@@ -1,0 +1,74 @@
+Require Import cliqueColorable.    
+
+Theorem validEnvDomainUnique : forall Gamma C eta' eta i U, 
+                                 valid Gamma C i eta' eta ->
+                                 (forall x, Ensembles.In _ U x -> x > 3 * i + 2) -> 
+                                 genericUnique U (fun a => match a with (x,y) => x end) eta'. 
+Proof.
+  intros. genDeps {{ U }}. induction H; intros. 
+  {constructor. constructor. constructor. eapply IHvalid. intros. inv H3.
+   inv H4. inv H1. apply H2 in H3. omega. inv H3. omega. inv H1. omega. inv H4. omega.
+   intros c. inv c. inv H3. apply H2 in H1. omega. inv H1. omega. inv H3. omega. 
+   intros c. inv c. apply H2 in H3. omega. inv H3. omega. intros c. apply H2 in c. omega. }
+  {constructor. constructor. constructor. eapply IHvalid. intros. inv H3.
+   inv H4. inv H1. apply H2 in H3. omega. inv H3. omega. inv H1. omega. inv H4. omega.
+   intros c. inv c. inv H3. apply H2 in H1. omega. inv H1. omega. inv H3. omega. 
+   intros c. inv c. apply H2 in H3. omega. inv H3. omega. intros c. apply H2 in c. omega. }
+  {constructor. }
+Qed. 
+
+Theorem KColorNPC : forall Gamma Delta F C eta G eta' S1 S2 S3 S4 U,
+                      reduce Gamma Delta F C G -> uniqueLockstep S1 S2 S3 S4 Gamma ->
+                      valid Gamma C 1 eta' eta -> genericUnique U (fun x => x) Delta -> 
+                      (SAT' eta F <-> coloring eta' G C).
+Proof. 
+  intros. inv H. split; intros. 
+  {constructor. admit. constructor. copy H1. 
+   apply validEnvDomainUnique with (U:=Empty_set _) in H1. Focus 2. intros. 
+   inv H7. eapply cliqueColorable; eauto. admit. }
+  {Admitted. 
+
+
+Theorem buildCtxtUnique : forall n Gamma Delta U, 
+                            (Gamma, Delta) = buildCtxt n -> 
+                            (forall x, Ensembles.In vvar U x -> x > n) -> 
+                            genericUnique U (fun x=> x) Delta. 
+Proof.
+  induction n; intros. 
+  {simpl in *. inv H. constructor. }
+  {simpl in *. destruct (buildCtxt n). invertTupEq. constructor.
+   eapply IHn; eauto. intros. inv H. apply H0 in H1. omega. inv H1. omega. 
+   intros c. apply H0 in c. omega. }
+Qed. 
+
+Theorem buildCtxtUniqueLS : forall n Gamma Delta S1 S2 S3 S4, 
+                              (Gamma, Delta) = buildCtxt n -> 
+                              (forall x, Ensembles.In vvar S1 x -> x > n) ->
+                              (forall x, Ensembles.In vvar S2 x -> x > 3*n) ->
+                              (forall x, Ensembles.In vvar S3 x -> x > 3*n+1) ->
+                              (forall x, Ensembles.In vvar S4 x -> x > 3*n+2) ->
+                              uniqueLockstep S1 S2 S3 S4 Gamma.
+Proof.
+  induction n; intros. 
+  {simpl in *. invertTupEq. repeat econstructor. }
+  {simpl in *. destruct (buildCtxt n) eqn:eq. invertTupEq. constructor. 
+   eapply IHn; auto. intros; inv H;[apply H0 in H4; omega|inv H4;omega].
+   intros; inv H; [apply H1 in H4; omega|inv H4;omega].  
+   intros; inv H;[apply H2 in H4; omega|inv H4;omega]. 
+   intros; inv H;[apply H3 in H4; omega|inv H4;omega]. 
+   intros c. apply H0 in c. omega. intros c. apply H1 in c. omega. intros c. 
+   apply H2 in c. omega. intros c. apply H3 in c. omega. }
+Qed. 
+
+Theorem KColorNPCTopLevel : forall Gamma Delta F n G eta eta', 
+                              (Gamma, Delta) = buildCtxt n ->
+                              reduce Gamma Delta F (n+1) G -> valid Gamma (n+1) 1 eta' eta ->
+                              (SAT' eta F <-> coloring eta' G (n+1)). 
+Proof.
+  intros. copy H. apply buildCtxtUnique with (U:=Empty_set _) in H. Focus 2. intros. 
+  inv H3. eapply buildCtxtUniqueLS with (S1:=Empty_set _)(S2:=Empty_set _)
+          (S3:=Empty_set _)(S4:=Empty_set _) in H2; try solve[intros c1 c2; inv c2].
+  eapply KColorNPC in H0; eauto. 
+Qed. 
+
+
